rename node for easy reading

ver2_qbft_Style/Invariants.dfy
@@ -7,6 +7,28 @@ module M_Invariants {
     import opened M_System
 
 
+
+    /**
+     * Invariant: Constant fields kept by the system, e.g. Node counts(Honest & Byzantine), Node role(Honest always be honest?)
+     */
+    ghost predicate inv_Constant_Fields(ss : SystemState)
+    // {
+    // }
+
+    /**
+     * Invariant: All Blockchain should be consistent by its own. Consistency -> the former block should be parent of the later block.
+     */
+    ghost predicate inv_Blockchain_Inner_Consistency(b : Blockchain)
+    {
+        forall i1, i2 | i1 == i2-1 // TODO: Could be to strong
+                      ::
+                        && b[i1] == b[i2].parent
+    }
+
+
+    /**
+     * Invariant: Each honest node are forced to vote PROPOSAL only one time at the same view. See Page(6): PROOF of Lemma 1
+     */
     ghost predicate inv_Honest_Node_Only_Vote_One_Proposal_At_Same_View(ss : SystemState)
     {
         forall r | IsHonest(ss, r) ::
@@ -23,6 +45,10 @@ module M_Invariants {
                             m1 == m2
     }
 
+
+    /**
+     * Invariant: Each honest node are forced to vote only one PREPARE message from leader at the same view. See Page(6): PROOF of Lemma 1
+     */
     ghost predicate inv_Honest_Node_Only_Vote_One_Prepare_At_Same_View(ss : SystemState)
     {
         forall r | IsHonest(ss, r) ::
@@ -39,6 +65,10 @@ module M_Invariants {
                             m1 == m2
     }
 
+
+    /**
+     * Invariant: Each honest node are forced to vote only one PRECOMMIT message from leader at the same view. See Page(6): PROOF of Lemma 1
+     */
     ghost predicate inv_Honest_Node_Only_Vote_One_PreCommit_At_Same_View(ss : SystemState)
     {
         forall r | IsHonest(ss, r) ::
@@ -53,6 +83,16 @@ module M_Invariants {
                             && m1.viewNum == m2.viewNum
                           ::
                             m1 == m2
+    }
+
+    ghost predicate inv_Honest_Node_Commit_Not_Conflict_Block(ss : SystemState)
+    {
+        forall r1, r2 | 
+                        && IsHonest(ss, r1)
+                        && IsHonest(ss, r2)
+                      ::
+                        && NoConflict(ss.nodeStates[r1].commitQC.block, ss.nodeStates[r2].commitQC.block)   //TODO: define block confliction
+            
     }
 
 }
